theories/typing/bool.v
@@ -31,6 +31,24 @@ Section bool.
     iIntros. iApply type_let; [apply type_bool_instr|solve_typing|done..].
   Qed.
 
+  Lemma type_nd_bool_instr E L :
+    typed_instr_ty E L +[] NdBool bool_ty (λ post '-[], ∀b, post b).
+  Proof.
+    iIntros (???) "_ _ _ _ _ $$ _ #?". iMod persistent_time_receipt_0 as "⧖".
+    wp_nd_int z. wp_op. iExists -[const _]. rewrite right_id tctx_hasty_val'; [|done].
+    iSplit. { iExists _. iFrame "⧖". by iExists _. }
+    by iApply proph_obs_impl; [|done]=>/= ??.
+  Qed.
+
+  Lemma type_nd_bool {𝔄l 𝔅} (T: tctx 𝔄l) x e tr E L (C: cctx 𝔅) :
+    Closed (x :b: []) e →
+    (∀v: val, typed_body E L C (v ◁ bool_ty +:: T) (subst' x v e) tr) -∗
+    typed_body E L C T (let: x := NdBool in e)
+      (λ post al, ∀b, tr post (b -:: al))%type.
+  Proof.
+    iIntros. by iApply type_let; [apply type_nd_bool_instr|solve_typing| |done].
+  Qed.
+
   Lemma type_if {𝔄l 𝔅l ℭ} p (T: tctx 𝔄l) (T': tctx 𝔅l) e1 e2 tr1 tr2 trx E L (C: cctx ℭ) :
     tctx_extract_ctx E L +[p ◁ bool_ty] T T' trx →
     typed_body E L C T' e1 tr1 -∗ typed_body E L C T' e2 tr2 -∗
