theories/util/basic.v
@@ -127,13 +127,6 @@ Fixpoint forall2b (xl: list A) (yl: list B) :=
   end.
 End forall2b.
 
-Definition list_to_option {A} (xl: list A) : option (A * list A) :=
-  match xl with [] => None | x :: xl' => Some (x, xl') end.
-Definition option_to_list {A} (o: option (A * list A)) : list A :=
-  match o with None => [] | Some (x, xl') => x :: xl' end.
-Global Instance list_option_iso {A} : Iso (@option_to_list A) list_to_option.
-Proof. split; fun_ext; case=>//; by case. Qed.
-
 (** * Utility for [fin] *)
 
 Class IntoFin {n} (k: nat) (i: fin n) := into_fin: k = i.
